moved general properties of PF into separate file

fairness/lawyer/obligations/obls_termination.v
@@ -4,7 +4,7 @@ From stdpp Require Import namespaces.
 From iris.proofmode Require Import tactics.
 From iris.algebra Require Import gset gmultiset.
 From trillium.fairness Require Import locales_helpers inftraces fairness trace_len.
-From trillium.fairness.lawyer.obligations Require Import obligations_model multiset_utils obls_utils wf_utils.
+From trillium.fairness.lawyer.obligations Require Import obligations_model multiset_utils obls_utils wf_utils obls_pf.
 From stdpp Require Import relations.
 
 
@@ -12,22 +12,6 @@ Section Termination.
   Context `(OP: ObligationsParams Degree Level Locale LIM_STEPS).
   Context `{Countable Locale}. 
   Let OM := ObligationsModel OP.
-
-  Definition loc_step_no_exp_all δ1 τ δ2 :=
-    (exists π δ, burns_cp OP δ1 τ δ2 π δ) \/
-    (exists π δ δ' n, exchanges_cp OP δ1 τ δ2 π δ δ' n) \/
-    (exists l, creates_signal OP δ1 τ δ2 l) \/
-    (exists s, sets_signal OP δ1 τ δ2 s) \/
-    (exists s π δ δ', creates_ep OP δ1 τ δ2 s π δ δ').
-
-  Lemma loc_step_split δ1 τ δ2:
-    loc_step OP δ1 τ δ2 <->
-      (loc_step_no_exp_all δ1 τ δ2 \/ (exists sid π d, expects_ep OP δ1 τ δ2 sid π d)).
-  Proof using.
-    rewrite /loc_step_no_exp_all. split.
-    - intros [T|[T|[T|[T|[T|T]]]]]; tauto.
-    - intros [[T|[T|[T|[T|T]]]] | ?]; red; tauto.
-  Qed. 
 
   Section SignalsEventuallySet.
     Context (tr: obls_trace OP).
@@ -64,217 +48,16 @@ Section Termination.
       eapply NEVER. lia. 
     Qed.
       
-    Definition approx_expects (k: nat) (eps: gset (@ExpectPermission Degree)) :=
-      ([^op set] ep ∈ eps, let '(sid, π, d) := ep in
-        ((LIM_STEPS + 2) * set_before sid - k) *: {[+ d +]} ).
-
-    Instance cmp_phase'_dec: forall (x y: Phase * Degree),
-        Decision (phase_le x.1 y.1).
-    Proof using.
-      intros [??] [??]. simpl.
-      rewrite /phase_le. solve_decision.
-    Qed.
-
-    Local Instance cmp_phase'_dec' π0:
-      ∀ x : Phase * Degree, Decision ((λ '(π, _), phase_le π π0) x). 
-    Proof using.
-      intros [??]. simpl.
-      rewrite /phase_le. solve_decision.
-    Qed.
-
-    Local Instance cmp_phase'_dec'' π0:
-      ∀ x : SignalId * Phase * Degree, Decision ((λ '(_, π, _), phase_le π π0) x).
-    Proof using.
-      intros [[??]?]. rewrite /phase_le. solve_decision.
-    Qed. 
-
-    Definition PF' (P: Phase -> Prop)
-      `{forall π, Decision (P π)}
-      (k: nat) (δ: ProgressState OP) :=
-      (mset_map snd ∘ (mset_filter (fun '(π_, _) => P π_)) ∘ (ps_cps OP)) δ
-        ⊎
-      approx_expects k (filter (fun '(_, π_, _) => P π_) (ps_eps OP δ)).
-
     Definition phase_ge := flip phase_le. 
-    Definition PF (π: Phase) := PF' (phase_ge π). 
-
-    Definition TPF (P: Phase -> Prop)
-      `{forall π, Decision (P π)}
-      (i: nat): gmultiset Degree :=
-      from_option (PF' P ((LIM_STEPS + 2) * i)) ∅ (tr S!! i).
-
-    Lemma ms_le_exp_mono m n X Y
-      (LE: m <= n)
-      (SUB: X ⊆ Y)
-      :
-      ms_le deg_le (approx_expects n X) (approx_expects m Y).
-    Proof using.
-      clear -LE SUB. 
-      rewrite /approx_expects.
-      apply union_difference_L in SUB. rewrite SUB.
-      rewrite big_opS_union; [| set_solver].
-      etrans.
-      2: { rewrite gmultiset_op. apply ms_le_sub. 
-           apply gmultiset_disj_union_subseteq_l. }      
-      eapply big_opS_ms_le. intros [[??]?].
-      apply ms_le_sub.
-      apply scalar_mul_le. lia.
-    Qed.
-
-    Lemma ms_le_PF_le m n (* π *) P δ
-      `{forall π, Decision (P π)}
-      (LE: m <= n):
-      ms_le deg_le (PF' P n δ) (PF' P m δ).
-    Proof using.
-      apply ms_le_disj_union.
-      + apply ms_le_sub. apply mset_map_sub. apply mset_filter_subseteq_mono. mss.
-      + apply ms_le_exp_mono; [lia | reflexivity].
-    Qed. 
-
-    Lemma approx_expects_add k eps e 
-      (FRESH: e ∉ eps):
-      let n := ((LIM_STEPS + 2) * set_before (fst $ fst e) - k) in
-      approx_expects k (eps ∪ {[ e ]}) = approx_expects k eps ⊎ n *: {[+ e.2 +]}.
-    Proof using.
-      rewrite (union_comm_L _ {[ e ]}).
-      rewrite /approx_expects.
-      rewrite -leibniz_equiv_iff. 
-      rewrite big_opS_insert; auto.
-      rewrite gmultiset_op gmultiset_disj_union_comm. f_equiv.
-      destruct e as [[??]?]. done.
-    Qed.
-
-    Lemma exchange_cp_ms_le (* π__ow *)P δ1 τ δ2 k π d d' n
-      `{forall π, Decision (P π)}
-      (EXC: exchanges_cp OP δ1 τ δ2 π d d' n):
-      ms_le deg_le (PF' P (S k) δ2) (PF' P k δ1).
-    Proof using.
-      clear -EXC. rewrite /PF /PF'. 
-      inversion EXC; subst. 
-      destruct δ1. simpl in *. 
-      apply ms_le_disj_union.
-      + subst new_cps0.
-        rewrite !mset_filter_disj_union mset_map_disj_union.
-        rewrite !mset_filter_difference. 
-        rewrite !mset_filter_mul_comm.
-        rewrite !mset_filter_singleton. 
-        destruct decide.
-        2: { (* rewrite decide_False; [| tauto]. *)
-             rewrite multiset_difference_empty gmultiset_scalar_mul_empty.
-             rewrite mset_map_empty.
-             eapply ms_le_Proper; [reflexivity | | reflexivity].
-             mss. }
-        (* rewrite decide_True; [| tauto]. *)
-        rewrite mset_map_sub_diff. 
-        2: { apply gmultiset_singleton_subseteq_l.
-             by apply mset_filter_spec. }
-        rewrite mset_map_mul !mset_map_singleton. simpl.
-        apply ms_le_exchange.
-        * apply _. 
-        * eapply elem_of_mset_map. eexists (_, _). split; eauto.
-          apply mset_filter_spec. split; eauto. 
-        * done. 
-      + apply ms_le_exp_mono; [lia | reflexivity].
-    Qed.
-
-    Lemma create_ep_ms_le (* π__ow *) P δ1 τ δ2 k s π d d'
-      `{forall π, Decision (P π)}
-      (CREATE: creates_ep OP δ1 τ δ2 s π d d'):
-      ms_le deg_le (PF' P (S k) δ2) (PF' P k δ1).
-    Proof using.
-      clear -CREATE. 
-      rewrite /PF /PF'. inversion CREATE; subst.
-      destruct δ1. simpl in *.
-      subst new_cps0 new_eps0.
-      
-      rewrite !mset_filter_difference. 
-      rewrite !mset_filter_singleton.        
-      rewrite filter_union_L.
-      destruct decide.
-      2: { rewrite filter_singleton_not_L; [| tauto].
-           rewrite multiset_difference_empty. rewrite union_empty_r_L.
-           apply ms_le_disj_union.
-           + apply ms_le_sub. reflexivity. 
-           + apply ms_le_exp_mono; [lia | reflexivity]. }
-      
-      rewrite filter_singleton_L; [| tauto]. 
-      
-      rewrite mset_map_sub_diff. 
-      2: { apply gmultiset_singleton_subseteq_l.
-           by apply mset_filter_spec. }
-      rewrite mset_map_singleton. simpl.
-      
-      destruct (decide ((s, π, d') ∈ ps_eps)).
-      { rewrite union_comm_L subseteq_union_1_L; [| set_solver].
-        apply ms_le_disj_union.
-        + apply ms_le_sub. mss. 
-        + apply ms_le_exp_mono; [lia | reflexivity]. }
-      
-      forward eapply (approx_expects_add (S k)) as ->.
-      { by intros [??]%elem_of_filter. } 
-      rewrite (gmultiset_disj_union_comm _ ((_ - _) *: _)) gmultiset_disj_union_assoc. 
-      apply ms_le_disj_union; revgoals. 
-      + apply ms_le_exp_mono; [lia | reflexivity].
-      + simpl. apply ms_le_exchange.
-        * apply _. 
-        * eapply elem_of_mset_map. eexists (_, _). split; eauto.
-          apply mset_filter_spec. split; eauto. 
-        * done.
-    Qed.
-
-    Lemma loc_step_no_exp_all_ms_le (* π__ow *) P δ1 τ δ2 k
-      `{forall π, Decision (P π)}
-      (STEP: loc_step_no_exp_all δ1 τ δ2)
-      :
-      ms_le deg_le (PF' P (S k) δ2) (PF' P k δ1).
-    Proof using.
-      clear -STEP OM.
-      destruct STEP as [T|[T|[T|[T|T]]]]. 
-      - destruct T as (?&?&T). inversion T; subst. 
-        destruct δ1. simpl in *.
-        apply ms_le_disj_union.
-        + apply ms_le_sub. apply mset_map_sub. apply mset_filter_subseteq_mono. mss.
-        + apply ms_le_exp_mono; [lia | reflexivity].
-      - destruct T as (?&?&?&?&T).
-        eapply exchange_cp_ms_le; eauto. 
-      - destruct T as (?&T). inversion T; subst.
-        destruct δ1. simpl in *.
-        apply ms_le_disj_union.
-        + apply ms_le_sub. apply mset_map_sub. mss. 
-        + apply ms_le_exp_mono; [lia | reflexivity].
-      - destruct T as (?&T). inversion T; subst.
-        destruct δ1. simpl in *.  
-        apply ms_le_disj_union.
-        + apply ms_le_sub. apply mset_map_sub. mss. 
-        + apply ms_le_exp_mono; [lia | reflexivity].
-      - destruct T as (?&?&?&?&T). eapply create_ep_ms_le; eauto. 
-    Qed.
-
-    Definition expect_ms_le (* π *) P δ1 τ δ2 k
-      `{forall π, Decision (P π)}:=
-      forall sid π' d,
-        expects_ep _ δ1 τ δ2 sid π' d ->
-        ms_le deg_le (PF' P (S k) δ2) (PF' P k δ1). 
-
-    Lemma loc_step_ms_le (* π *) P δ1 τ δ2 k
-      `{forall π, Decision (P π)}
-      (STEP: loc_step _ δ1 τ δ2)
-      (EXP_CASE: expect_ms_le P δ1 τ δ2 k)
-      :
-      ms_le deg_le (PF' P (S k) δ2) (PF' P k δ1).
-    Proof using.
-      clear LVL_WF.
-      apply loc_step_split in STEP as [NOEXP | EXP].
-      - eapply loc_step_no_exp_all_ms_le; eauto.
-      - destruct EXP as (?&?&?&?). eapply EXP_CASE; eauto.
-    Qed.
+    Definition PF (π: Phase) := PF' OP set_before (phase_ge π).
+    Definition TPF (π: Phase) := TPF' OP tr set_before (phase_ge π).
 
     Let π0 := nroot. 
 
     Lemma other_expect_ms_le π__ow δ1 τ δ2 k
       (OTHER: let π := default π0 (ps_phases _ δ1 !! τ) in
               phases_incompat π__ow π):
-      expect_ms_le (phase_ge π__ow) δ1 τ δ2 k. 
+      expect_ms_le OP set_before (phase_ge π__ow) δ1 τ δ2 k. 
     Proof using.
       clear LVL_WF SET_BEFORE_SPEC. 
       red. intros sid π' d EXP. 
@@ -300,7 +83,7 @@ Section Termination.
                   k < n)
       :
       let π__ow := default π0 (ps_phases _ δ1 !! τ) in
-      expect_ms_le (phase_ge π__ow) δ1 τ δ2 k. 
+      expect_ms_le OP set_before (phase_ge π__ow) δ1 τ δ2 k. 
     Proof using.
       clear LVL_WF SET_BEFORE_SPEC.
       intros. red. intros sid π' d EXP. 
@@ -337,113 +120,22 @@ Section Termination.
       rewrite -gmultiset_scalar_mul_S_r. f_equiv. lia.
     Qed.
 
-    Definition nsteps_keep_ms_le (* π *) P δ i τ
-      `{forall π, Decision (P π)}
-      :=
-      forall δ' k
-      (ITH: tr S!! i = Some δ)
-      (BOUND : k ≤ LIM_STEPS)
-      (STEPS: nsteps (λ p1 p2, loc_step OP p1 τ p2) k δ δ'),
-      ms_le deg_le (PF' P ((LIM_STEPS + 2) * i + k) δ') (PF' P ((LIM_STEPS + 2) * i) δ).
-
-    Lemma forks_locale_ms_le (* π *) P δ1 τ δ2 τ' R k
-      `{forall π, Decision (P π)}
-      (FORK: forks_locale OP δ1 τ δ2 τ' R):
-      ms_le deg_le (PF' P (S k) δ2) (PF' P k δ1).
-    Proof using.
-      rewrite /PF.
-      inversion FORK; subst. 
-      destruct δ1. simpl in *.
-      apply ms_le_disj_union.
-      + apply ms_le_sub. apply mset_map_sub. mss. 
-      + apply ms_le_exp_mono; [lia | reflexivity].
-    Qed.
-
-    Lemma om_trans_ms_rel (bd: bool) (* π *) P i
-      `{forall π, Decision (P π)}
-      (rel := (if bd then ms_lt deg_le else ms_le deg_le): relation (gmultiset Degree))
-      (VALID: obls_trace_valid OP tr)
-      (BURN_REL:
-        forall δ δ' τ mb mf k,
-          tr !! i = Some (δ, Some (τ, δ')) ->
-          k ≤ LIM_STEPS ->
-          nsteps (λ p1 p2, loc_step OP p1 τ p2) k δ mb ->
-          (∃ π δ, burns_cp OP mb τ mf π δ) ->
-          clos_refl (ProgressState OP) (λ p1 p2, ∃ τ' R, forks_locale OP p1 τ p2 τ' R) mf δ' ->
-          rel (PF' P ((LIM_STEPS + 2) * i + LIM_STEPS + 1) mf) (PF' P ((LIM_STEPS + 2) * i + LIM_STEPS) mb))
-      (NSTEPS_LE: forall δ τ,
-          tr L!! i = Some τ ->
-          nsteps_keep_ms_le P δ i τ)
-      (DOM: is_Some (tr S!! (S i))):
-      rel (TPF P (S i)) (TPF P i).
-    Proof using.
-      rewrite /TPF. simpl.
-      forward eapply (proj2 (label_lookup_states' _ _)) as [τ ITHl]; eauto.  
-      forward eapply (state_lookup_prev _ _ DOM _ (PeanoNat.Nat.le_succ_diag_r _)).
-      intros [δ ITH]. destruct DOM as [δ' ITH']. rewrite ITH ITH'. simpl. 
-
-      forward eapply trace_valid_steps'' as STEP; eauto.
-      { rewrite Nat.add_1_r. eauto. }
-      simpl in STEP. red in STEP. destruct STEP as (mf & PSTEP & FSTEP).
-      red in PSTEP. destruct PSTEP as (k & BOUND & (mb & PSTEP & BSTEP)).
-
-      eapply BURN_REL in BSTEP; eauto.
-      2: { eapply state_label_lookup; eauto. rewrite Nat.add_1_r. eauto. }
-      eapply NSTEPS_LE in PSTEP; eauto. 
-
-      assert (ms_le deg_le (PF' P ((LIM_STEPS + 2) * S i) δ')
-            (PF' P ((LIM_STEPS + 2) * i + LIM_STEPS + 1) mf)) as LE. 
-      { inversion FSTEP as [? FORK | ]. 
-        2: { subst mf.
-             rewrite /PF. apply ms_le_disj_union.
-             - reflexivity.
-             - apply ms_le_exp_mono; [lia | reflexivity]. }
-        destruct FORK as (?&?&?). 
-        subst y. eapply ms_le_Proper; [| reflexivity| eapply forks_locale_ms_le; eauto].
-        f_equiv. apply leibniz_equiv_iff. lia. }  
-
-      destruct bd; subst rel.
-      - eapply strict_transitive_l; [| apply PSTEP]. 
-        eapply strict_transitive_r; [apply LE| ]. 
-        eapply strict_transitive_l; [apply BSTEP| ].
-        apply ms_le_PF_le. lia.
-      - etrans; [| apply PSTEP].
-        etrans; [apply LE| ].
-        etrans; [apply BSTEP| ].
-        apply ms_le_PF_le. lia.
-    Qed.
-
     Lemma never_set_owned s c
       (NEVER_SET: never_set_after s c):
       forall i, c <= i ->
            map_Exists (fun τ obs => s ∈ obs) (from_option (ps_obls _) ∅ (tr S!! i)). 
     Proof using OM. Admitted. 
 
-    Lemma burns_cp_ms_le δ1 τ δ2 (* π *) P π' d k
-      `{forall π, Decision (P π)}
-      (STEP: burns_cp OP δ1 τ δ2 π' d):
-      ms_le deg_le (PF' P (S k) δ2) (PF' P k δ1).
-    Proof using.
-      clear LVL_WF SET_BEFORE_SPEC. 
-      rewrite /PF. 
-      inversion STEP; subst.
-      destruct δ1. simpl in *.
-      apply ms_le_disj_union.
-      + apply ms_le_sub. apply mset_map_sub.
-        apply mset_filter_subseteq_mono. mss. 
-      + apply ms_le_exp_mono; [lia | reflexivity].
-    Qed.        
-
     Lemma other_om_trans_ms_le πτ τ n
       (VALID: obls_trace_valid OP tr)
       (PH: from_option (fun δ => ps_phases _ δ !! τ = Some πτ) False (tr S!! n))
       (NOτ: tr L!! n ≠ Some τ):
-      ms_le deg_le (TPF (phase_ge πτ) (S n)) (TPF (phase_ge πτ) n).
+      ms_le deg_le (TPF πτ (S n)) (TPF πτ n).
     Proof using.
       destruct (tr S!! (S n)) as [δ'| ] eqn:NEXT.
-      2: { rewrite /TPF. rewrite NEXT. simpl. apply empty_ms_le. }
+      2: { rewrite /TPF /TPF'. rewrite NEXT. simpl. apply empty_ms_le. }
      
-      apply (om_trans_ms_rel false); auto.
+      eapply om_trans_ms_rel with (bd := false); auto.
       { intros.
         rewrite Nat.add_succ_r. rewrite Nat.add_0_r.  
         destruct H4 as (?&?&?). eapply burns_cp_ms_le; eauto. }
@@ -486,7 +178,7 @@ Section Termination.
       (PH: ps_phases _ δ0 !! τ = Some π)
       (LE: i <= j)
       (NOτ: forall k, i <= k < j -> tr L!! k ≠ Some τ):
-      ms_le deg_le (TPF (phase_ge π) j) (TPF (phase_ge π) i).
+      ms_le deg_le (TPF π j) (TPF π i).
     Proof using. 
       apply Nat.le_sum in LE as [d ->]. induction d.
       { rewrite Nat.add_0_r. reflexivity. }
@@ -496,7 +188,7 @@ Section Termination.
       rewrite -plus_n_Sm.
 
       destruct (tr S!! (S (i + d))) as [δ'| ] eqn:NEXT.
-      2: { rewrite /TPF. rewrite NEXT. simpl. apply empty_ms_le. }
+      2: { rewrite /TPF /TPF'. rewrite NEXT. simpl. apply empty_ms_le. }
       forward eapply (state_lookup_prev _ _ ltac:(eauto) _ (PeanoNat.Nat.le_succ_diag_r _)).
       intros [δ IDTH].
 
@@ -553,42 +245,6 @@ Section Termination.
       edestruct @strict_not_both; eauto. 
     Admitted.
 
-    Lemma burns_cp_own_ms_lt δ1 τ δ2 πτ πb d k P
-      `{forall π, Decision (P π)}
-      (PH: ps_phases _ δ1 !! τ = Some πτ)
-      (Pτ: P πb)
-      (STEP: burns_cp OP δ1 τ δ2 πb d):
-      ms_lt deg_le (PF' P (S k) δ2) (PF' P k δ1).
-    Proof using.
-      clear tr SET_BEFORE_SPEC LVL_WF.
-      rewrite /PF /PF'. 
-      inversion STEP; subst.
-      destruct δ1. simpl in *.
-
-      eapply ms_le_lt_disj_union. 
-      2: { apply ms_le_exp_mono; [ | reflexivity]. apply Nat.le_succ_diag_r. }
-      
-      apply strict_spec_alt.
-      
-      split. 
-      { apply ms_le_sub. apply mset_map_sub.
-        apply mset_filter_subseteq_mono. mss. }
-      rewrite mset_filter_difference mset_filter_singleton.  
-      rewrite mset_map_sub_diff. 
-
-      2: { rewrite decide_True.
-           2: { set_solver. }
-           apply gmultiset_singleton_subseteq_l.
-           apply mset_filter_spec. split; [done| ]. set_solver. }
-      rewrite decide_True; [| set_solver]. 
-      rewrite mset_map_singleton. simpl.
-      apply gmultiset_disj_union_difference' in CP. rewrite CP.
-      
-      rewrite mset_filter_disj_union mset_filter_singleton decide_True; [| set_solver].
-      rewrite mset_map_disj_union mset_map_singleton. simpl.
-      mss. 
-    Qed.
-
     Lemma owm_om_trans_ms_lt πτ τ n s δ0
       (NTH: tr S!! n = Some δ0)
       (VALID: obls_trace_valid OP tr)
@@ -597,11 +253,11 @@ Section Termination.
       (MIN: minimal_in_prop tr_sig_lt (s, n) (λ sn, never_set_after sn.1 sn.2))
       (OWNER: s ∈ default ∅ (ps_obls _ δ0 !! τ))
       (LBL: tr L!! n = Some τ):
-      ms_lt deg_le (TPF (phase_ge πτ) (S n)) (TPF (phase_ge πτ) n).
+      ms_lt deg_le (TPF πτ (S n)) (TPF πτ n).
     Proof using.
       forward eapply (proj1 (label_lookup_states' _ _)); eauto. intros [δ' NTH']. 
       
-      apply (om_trans_ms_rel true); auto.
+      eapply om_trans_ms_rel with (bd := true); auto.
       { intros.
         rewrite Nat.add_succ_r Nat.add_0_r.
         apply state_label_lookup in H1 as (NTH_&?&LBL_).
@@ -657,6 +313,7 @@ Section Termination.
     Admitted.
 
     Let any_phase (_: Phase) := True.
+    Definition APF := TPF' OP tr set_before any_phase.
 
     (* TODO: move *)
     Lemma gset_filter_True `{Countable K} (g: gset K)
@@ -671,7 +328,7 @@ Section Termination.
                   let n := (LIM_STEPS + 2) * set_before sid in
                   k < n)
       :
-      expect_ms_le any_phase δ1 τ δ2 k. 
+      expect_ms_le OP set_before any_phase δ1 τ δ2 k. 
     Proof using SET_BEFORE_SPEC.
       clear LVL_WF.
       intros. red. intros sid π' d EXP. 
@@ -716,11 +373,11 @@ Section Termination.
       (* (LBL: tr L!! n = Some τ) *)
       (DOM: is_Some (tr S!! (S n)))
       :
-      ms_lt deg_le (TPF any_phase (S n)) (TPF any_phase n).
+      ms_lt deg_le (APF (S n)) (APF n).
     Proof using.
       destruct DOM as [δ' NTH']. 
       
-      apply (om_trans_ms_rel true); auto.
+      eapply om_trans_ms_rel with (bd := true); auto.
       { intros δ δ'_ τ mb mf k NTH BOUND PSTEPS BURNS FORKS. 
         rewrite Nat.add_succ_r Nat.add_0_r.
         apply state_label_lookup in NTH as (NTH_&NTH'_&LBL_).
@@ -863,7 +520,7 @@ Section Termination.
       (UNSET: never_set_after s c)
       (MIN: minimal_in_prop tr_sig_lt (s, c)
           (λ ab : SignalId * nat, never_set_after ab.1 ab.2))
-      (OTF := λ i, TPF (phase_ge (s_ow s i)) i):
+      (OTF := λ i, TPF (s_ow s i) i):
       ∀ d, c ≤ d → ∃ j, d < j ∧ ms_lt deg_le (OTF j) (OTF d).
     Proof using.
       intros d LE.
@@ -929,7 +586,7 @@ Section Termination.
       
       intros LT.
       exists (S (d + m)). split; [lia| ].
-      rewrite /OTF. erewrite (S_OWNER _ d); eauto.
+      rewrite /OTF /TPF /TPF'. erewrite (S_OWNER _ d); eauto.
       2: { by rewrite OBLSd. }
       eapply strict_transitive_l; [| apply TPFle]. 
       eapply strict_transitive_r; [| apply LT].
@@ -957,10 +614,10 @@ Section Termination.
       2: { rewrite OBLSd'. done. } 
       
       (* TODO: extract? *)
-      rewrite /TPF.
+      rewrite /TPF /TPF' /PF'.
       generalize ((LIM_STEPS + 2) * S (d + m)) as N. intros.
       rewrite plus_n_Sm -Nat.add_1_r Nat.add_assoc MTH'. simpl.
-      rewrite /PF. apply ms_le_disj_union.
+      apply ms_le_disj_union.
       - apply ms_le_sub, mset_map_sub.
         apply mset_filter_subseteq_mono_strong.
         intros [pi de] IN' LEpi.
@@ -983,7 +640,7 @@ Section Termination.
       eapply sets_have_min in EX; [| apply tr_sig_lt_wf].
       apply ex_prod in EX. simpl in EX. destruct EX as (s & c & UNSET & MIN).
       
-      set (OTF i := TPF (phase_ge (s_ow s i)) i).
+      set (OTF i := TPF (s_ow s i) i).
 
       set (R := MR (ms_lt deg_le) (fun i => OTF (c + i))). 
       forward eapply well_founded_ind with (R := R) (P := fun _ => False).
