fairness/lawyer/obligations/obls_pf.v
@@ -1,0 +1,351 @@
+Require Import Relation_Operators.
+From iris.proofmode Require Import tactics.
+From iris.algebra Require Import gset gmultiset.
+From trillium.fairness Require Import inftraces trace_lookup.
+From trillium.fairness.lawyer.obligations Require Import obligations_model multiset_utils.
+From stdpp Require Import relations.
+
+
+Section PhaseFuel.
+  Context `(OP: ObligationsParams Degree Level Locale LIM_STEPS).
+  Context `{Countable Locale}. 
+  Let OM := ObligationsModel OP.
+
+  Definition loc_step_no_exp_all δ1 τ δ2 :=
+    (exists π δ, burns_cp OP δ1 τ δ2 π δ) \/
+    (exists π δ δ' n, exchanges_cp OP δ1 τ δ2 π δ δ' n) \/
+    (exists l, creates_signal OP δ1 τ δ2 l) \/
+    (exists s, sets_signal OP δ1 τ δ2 s) \/
+    (exists s π δ δ', creates_ep OP δ1 τ δ2 s π δ δ').
+
+  Lemma loc_step_split δ1 τ δ2:
+    loc_step OP δ1 τ δ2 <->
+      (loc_step_no_exp_all δ1 τ δ2 \/ (exists sid π d, expects_ep OP δ1 τ δ2 sid π d)).
+  Proof using.
+    rewrite /loc_step_no_exp_all. split.
+    - intros [T|[T|[T|[T|[T|T]]]]]; tauto.
+    - intros [[T|[T|[T|[T|T]]]] | ?]; red; tauto.
+  Qed.
+    
+  Context (tr: obls_trace OP).
+  
+  Context `{Inhabited Level}. 
+  Let lvl__def := @inhabitant Level _. 
+  
+  Context (sig_bound: SignalId -> nat).
+  
+  Definition approx_expects (k: nat) (eps: gset (@ExpectPermission Degree)) :=
+    ([^op set] ep ∈ eps, let '(sid, π, d) := ep in
+                         ((LIM_STEPS + 2) * sig_bound sid - k) *: {[+ d +]} ).
+  
+  Instance cmp_phase'_dec: forall (x y: Phase * Degree),
+      Decision (phase_le x.1 y.1).
+  Proof using.
+    intros [??] [??]. simpl.
+    rewrite /phase_le. solve_decision.
+  Qed.
+  
+  Local Instance cmp_phase'_dec' π0:
+    ∀ x : Phase * Degree, Decision ((λ '(π, _), phase_le π π0) x). 
+  Proof using.
+    intros [??]. simpl.
+    rewrite /phase_le. solve_decision.
+  Qed.
+  
+  Local Instance cmp_phase'_dec'' π0:
+    ∀ x : SignalId * Phase * Degree, Decision ((λ '(_, π, _), phase_le π π0) x).
+  Proof using.
+    intros [[??]?]. rewrite /phase_le. solve_decision.
+  Qed.
+
+  Context (P: Phase -> Prop).
+  Context `{forall π, Decision (P π)}. 
+  
+  Definition PF' (k: nat) (δ: ProgressState OP) :=
+    (mset_map snd ∘ (mset_filter (fun '(π_, _) => P π_)) ∘ (ps_cps OP)) δ
+      ⊎
+      approx_expects k (filter (fun '(_, π_, _) => P π_) (ps_eps OP δ)).
+  
+  Definition TPF' (i: nat): gmultiset Degree :=
+    from_option (PF' ((LIM_STEPS + 2) * i)) ∅ (tr S!! i).
+  
+  Lemma ms_le_exp_mono m n X Y
+    (LE: m <= n)
+    (SUB: X ⊆ Y)
+    :
+    ms_le deg_le (approx_expects n X) (approx_expects m Y).
+  Proof using.
+    clear -LE SUB. 
+    rewrite /approx_expects.
+    apply union_difference_L in SUB. rewrite SUB.
+    rewrite big_opS_union; [| set_solver].
+    etrans.
+    2: { rewrite gmultiset_op. apply ms_le_sub. 
+         apply gmultiset_disj_union_subseteq_l. }      
+    eapply big_opS_ms_le. intros [[??]?].
+    apply ms_le_sub.
+    apply scalar_mul_le. lia.
+  Qed.
+  
+  Lemma ms_le_PF_le m n δ
+    (LE: m <= n):
+    ms_le deg_le (PF' n δ) (PF' m δ).
+  Proof using.
+    apply ms_le_disj_union.
+    + apply ms_le_sub. apply mset_map_sub. apply mset_filter_subseteq_mono. mss.
+    + apply ms_le_exp_mono; [lia | reflexivity].
+  Qed. 
+  
+  Lemma approx_expects_add k eps e 
+    (FRESH: e ∉ eps):
+    let n := ((LIM_STEPS + 2) * sig_bound (fst $ fst e) - k) in
+    approx_expects k (eps ∪ {[ e ]}) = approx_expects k eps ⊎ n *: {[+ e.2 +]}.
+  Proof using.
+    rewrite (union_comm_L _ {[ e ]}).
+    rewrite /approx_expects.
+    rewrite -leibniz_equiv_iff. 
+    rewrite big_opS_insert; auto.
+    rewrite gmultiset_op gmultiset_disj_union_comm. f_equiv.
+    destruct e as [[??]?]. done.
+  Qed.
+  
+  Lemma exchange_cp_ms_le δ1 τ δ2 k π d d' n
+    `{forall π, Decision (P π)}
+    (EXC: exchanges_cp OP δ1 τ δ2 π d d' n):
+    ms_le deg_le (PF' (S k) δ2) (PF' k δ1).
+  Proof using.
+    clear -EXC. rewrite /PF'. 
+    inversion EXC; subst. 
+    destruct δ1. simpl in *. 
+    apply ms_le_disj_union.
+    + subst new_cps0.
+      rewrite !mset_filter_disj_union mset_map_disj_union.
+      rewrite !mset_filter_difference. 
+      rewrite !mset_filter_mul_comm.
+      rewrite !mset_filter_singleton. 
+      destruct decide.
+      2: { rewrite multiset_difference_empty gmultiset_scalar_mul_empty.
+           rewrite mset_map_empty.
+           eapply ms_le_Proper; [reflexivity | | reflexivity].
+           mss. }
+      rewrite mset_map_sub_diff. 
+      2: { apply gmultiset_singleton_subseteq_l.
+           by apply mset_filter_spec. }
+      rewrite mset_map_mul !mset_map_singleton. simpl.
+      apply ms_le_exchange.
+      * apply _. 
+      * eapply elem_of_mset_map. eexists (_, _). split; eauto.
+        apply mset_filter_spec. split; eauto. 
+      * done. 
+    + apply ms_le_exp_mono; [lia | reflexivity].
+  Qed.
+  
+  Lemma create_ep_ms_le δ1 τ δ2 k s π d d'
+    (CREATE: creates_ep OP δ1 τ δ2 s π d d'):
+    ms_le deg_le (PF' (S k) δ2) (PF' k δ1).
+  Proof using.
+    clear -CREATE. 
+    rewrite /PF'. inversion CREATE; subst.
+    destruct δ1. simpl in *.
+    subst new_cps0 new_eps0.
+    
+    rewrite !mset_filter_difference. 
+    rewrite !mset_filter_singleton.        
+    rewrite filter_union_L.
+    destruct decide.
+    2: { rewrite filter_singleton_not_L; [| tauto].
+         rewrite multiset_difference_empty. rewrite union_empty_r_L.
+         apply ms_le_disj_union.
+         + apply ms_le_sub. reflexivity. 
+         + apply ms_le_exp_mono; [lia | reflexivity]. }
+    
+    rewrite filter_singleton_L; [| tauto]. 
+    
+    rewrite mset_map_sub_diff. 
+    2: { apply gmultiset_singleton_subseteq_l.
+         by apply mset_filter_spec. }
+    rewrite mset_map_singleton. simpl.
+    
+    destruct (decide ((s, π, d') ∈ ps_eps)).
+    { rewrite union_comm_L subseteq_union_1_L; [| set_solver].
+      apply ms_le_disj_union.
+      + apply ms_le_sub. mss. 
+      + apply ms_le_exp_mono; [lia | reflexivity]. }
+    
+    forward eapply (approx_expects_add (S k)) as ->.
+    { by intros [??]%elem_of_filter. } 
+    rewrite (gmultiset_disj_union_comm _ ((_ - _) *: _)) gmultiset_disj_union_assoc. 
+    apply ms_le_disj_union; revgoals. 
+    + apply ms_le_exp_mono; [lia | reflexivity].
+    + simpl. apply ms_le_exchange.
+      * apply _. 
+      * eapply elem_of_mset_map. eexists (_, _). split; eauto.
+        apply mset_filter_spec. split; eauto. 
+      * done.
+  Qed.
+  
+  Lemma loc_step_no_exp_all_ms_le δ1 τ δ2 k
+    (STEP: loc_step_no_exp_all δ1 τ δ2)
+    :
+    ms_le deg_le (PF' (S k) δ2) (PF' k δ1).
+  Proof using.
+    clear -STEP OM.
+    destruct STEP as [T|[T|[T|[T|T]]]]. 
+    - destruct T as (?&?&T). inversion T; subst. 
+      destruct δ1. simpl in *.
+      apply ms_le_disj_union.
+      + apply ms_le_sub. apply mset_map_sub. apply mset_filter_subseteq_mono. mss.
+      + apply ms_le_exp_mono; [lia | reflexivity].
+    - destruct T as (?&?&?&?&T).
+      eapply exchange_cp_ms_le; eauto. 
+    - destruct T as (?&T). inversion T; subst.
+      destruct δ1. simpl in *.
+      apply ms_le_disj_union.
+      + apply ms_le_sub. apply mset_map_sub. mss. 
+      + apply ms_le_exp_mono; [lia | reflexivity].
+    - destruct T as (?&T). inversion T; subst.
+      destruct δ1. simpl in *.  
+      apply ms_le_disj_union.
+      + apply ms_le_sub. apply mset_map_sub. mss. 
+      + apply ms_le_exp_mono; [lia | reflexivity].
+    - destruct T as (?&?&?&?&T). eapply create_ep_ms_le; eauto. 
+  Qed.
+  
+  Definition expect_ms_le δ1 τ δ2 k
+    :=
+    forall sid π' d,
+      expects_ep _ δ1 τ δ2 sid π' d ->
+      ms_le deg_le (PF' (S k) δ2) (PF' k δ1). 
+  
+  Lemma loc_step_ms_le δ1 τ δ2 k
+    (STEP: loc_step _ δ1 τ δ2)
+    (EXP_CASE: expect_ms_le δ1 τ δ2 k)
+    :
+    ms_le deg_le (PF' (S k) δ2) (PF' k δ1).
+  Proof using.
+    apply loc_step_split in STEP as [NOEXP | EXP].
+    - eapply loc_step_no_exp_all_ms_le; eauto.
+    - destruct EXP as (?&?&?&?). eapply EXP_CASE; eauto.
+  Qed.
+  
+  Definition nsteps_keep_ms_le δ i τ
+    :=
+    forall δ' k
+      (ITH: tr S!! i = Some δ)
+      (BOUND : k ≤ LIM_STEPS)
+      (STEPS: nsteps (λ p1 p2, loc_step OP p1 τ p2) k δ δ'),
+      ms_le deg_le (PF' ((LIM_STEPS + 2) * i + k) δ') (PF' ((LIM_STEPS + 2) * i) δ).
+  
+  Lemma forks_locale_ms_le δ1 τ δ2 τ' R k
+    (FORK: forks_locale OP δ1 τ δ2 τ' R):
+    ms_le deg_le (PF' (S k) δ2) (PF' k δ1).
+  Proof using.
+    rewrite /PF'.
+    inversion FORK; subst. 
+    destruct δ1. simpl in *.
+    apply ms_le_disj_union.
+    + apply ms_le_sub. apply mset_map_sub. mss. 
+    + apply ms_le_exp_mono; [lia | reflexivity].
+  Qed.
+  
+  Lemma om_trans_ms_rel (bd: bool) i
+    (rel := (if bd then ms_lt deg_le else ms_le deg_le): relation (gmultiset Degree))
+    (VALID: obls_trace_valid OP tr)
+    (BURN_REL:
+      forall δ δ' τ mb mf k,
+        tr !! i = Some (δ, Some (τ, δ')) ->
+        k ≤ LIM_STEPS ->
+        nsteps (λ p1 p2, loc_step OP p1 τ p2) k δ mb ->
+        (∃ π δ, burns_cp OP mb τ mf π δ) ->
+        clos_refl (ProgressState OP) (λ p1 p2, ∃ τ' R, forks_locale OP p1 τ p2 τ' R) mf δ' ->
+        rel (PF' ((LIM_STEPS + 2) * i + LIM_STEPS + 1) mf) (PF' ((LIM_STEPS + 2) * i + LIM_STEPS) mb))
+    (NSTEPS_LE: forall δ τ,
+        tr L!! i = Some τ ->
+        nsteps_keep_ms_le δ i τ)
+    (DOM: is_Some (tr S!! (S i))):
+    rel (TPF' (S i)) (TPF' i).
+  Proof using.
+    rewrite /TPF'. simpl.
+    forward eapply (proj2 (label_lookup_states' _ _)) as [τ ITHl]; eauto.  
+    forward eapply (state_lookup_prev _ _ DOM _ (PeanoNat.Nat.le_succ_diag_r _)).
+    intros [δ ITH]. destruct DOM as [δ' ITH']. rewrite ITH ITH'. simpl. 
+    
+    forward eapply trace_valid_steps'' as STEP; eauto.
+    { rewrite Nat.add_1_r. eauto. }
+    simpl in STEP. red in STEP. destruct STEP as (mf & PSTEP & FSTEP).
+    red in PSTEP. destruct PSTEP as (k & BOUND & (mb & PSTEP & BSTEP)).
+    
+    eapply BURN_REL in BSTEP; eauto.
+    2: { eapply state_label_lookup; eauto. rewrite Nat.add_1_r. eauto. }
+    eapply NSTEPS_LE in PSTEP; eauto. 
+    
+    assert (ms_le deg_le (PF' ((LIM_STEPS + 2) * S i) δ')
+              (PF' ((LIM_STEPS + 2) * i + LIM_STEPS + 1) mf)) as LE. 
+    { inversion FSTEP as [? FORK | ]. 
+      2: { subst mf.
+           rewrite /PF'. apply ms_le_disj_union.
+           - reflexivity.
+           - apply ms_le_exp_mono; [lia | reflexivity]. }
+      destruct FORK as (?&?&?). 
+      subst y. eapply ms_le_Proper; [| reflexivity| eapply forks_locale_ms_le; eauto].
+      f_equiv. apply leibniz_equiv_iff. lia. }  
+    
+    destruct bd; subst rel.
+    - eapply strict_transitive_l; [| apply PSTEP]. 
+      eapply strict_transitive_r; [apply LE| ]. 
+      eapply strict_transitive_l; [apply BSTEP| ].
+      apply ms_le_PF_le. lia.
+    - etrans; [| apply PSTEP].
+      etrans; [apply LE| ].
+      etrans; [apply BSTEP| ].
+      apply ms_le_PF_le. lia.
+  Qed.
+  
+  Lemma burns_cp_ms_le δ1 τ δ2 π' d k
+    (STEP: burns_cp OP δ1 τ δ2 π' d):
+    ms_le deg_le (PF' (S k) δ2) (PF' k δ1).
+  Proof using.
+    rewrite /PF'. 
+    inversion STEP; subst.
+    destruct δ1. simpl in *.
+    apply ms_le_disj_union.
+    + apply ms_le_sub. apply mset_map_sub.
+      apply mset_filter_subseteq_mono. mss. 
+    + apply ms_le_exp_mono; [lia | reflexivity].
+  Qed.        
+  
+  Lemma burns_cp_own_ms_lt δ1 τ δ2 πτ πb d k
+    (PH: ps_phases _ δ1 !! τ = Some πτ)
+    (Pτ: P πb)
+    (STEP: burns_cp OP δ1 τ δ2 πb d):
+    ms_lt deg_le (PF' (S k) δ2) (PF' k δ1).
+  Proof using.
+    rewrite /PF'. 
+    inversion STEP; subst.
+    destruct δ1. simpl in *.
+    
+    eapply ms_le_lt_disj_union. 
+    2: { apply ms_le_exp_mono; [ | reflexivity]. apply Nat.le_succ_diag_r. }
+    
+    apply strict_spec_alt.
+    
+    split. 
+    { apply ms_le_sub. apply mset_map_sub.
+      apply mset_filter_subseteq_mono. mss. }
+    rewrite mset_filter_difference mset_filter_singleton.  
+    rewrite mset_map_sub_diff. 
+    
+    2: { rewrite decide_True.
+         2: { set_solver. }
+         apply gmultiset_singleton_subseteq_l.
+         apply mset_filter_spec. split; [done| ]. set_solver. }
+    rewrite decide_True; [| set_solver]. 
+    rewrite mset_map_singleton. simpl.
+    apply gmultiset_disj_union_difference' in CP. rewrite CP.
+    
+    rewrite mset_filter_disj_union mset_filter_singleton decide_True; [| set_solver].
+    rewrite mset_map_disj_union mset_map_singleton. simpl.
+    mss. 
+  Qed.
+  
+End PhaseFuel.
